Pdl.lean
@@ -6,9 +6,8 @@ import «Pdl».Vocab
 import «Pdl».Semantics
 import «Pdl».Star
 import «Pdl».Discon
--- import «Pdl».Unravel -- no longer used!
 import «Pdl».DagTableau
 import «Pdl».Tableau
 import «Pdl».Examples
-import «Pdl».Interpolation
 import «Pdl».Modelgraphs
+import «Pdl».Interpolation
